Update Imp_J.v

Imp_J.v
@@ -37,42 +37,31 @@
     命令型プログラムについての推論のための論理として一番知られているホーア論理
     (_Hoare Logic_)を紹介します。 *)
 
-(* ####################################################### *)
-(** *** Sflib *)
-
-(*  A minor technical point: Instead of asking Coq to import our
-    earlier definitions from chapter [Logic], we import a small library
-    called [Sflib.v], containing just a few definitions and theorems
-    from earlier chapters that we'll actually use in the rest of the
-    course.  This change should be nearly invisible, since most of what's
-    missing from Sflib has identical definitions in the Coq standard
-    library.  The main reason for doing it is to tidy the global Coq
-    environment so that, for example, it is easier to search for
-    relevant theorems. *)
-(** マイナーな技術的ポイント: ここまでの定義をLogic_J.vからインポートする代わりに、
-    Sflib_J.vという小さなライブラリをインポートします。 このライブラリは、
-    前の章の定義や定理のうち、残りの章で実際に使うものだけを集めたものです。 
-    読者はそれほど違うものとは感じないでしょう。というのは、 Sflib で抜けているものの
-    ほとんどは、Coqの標準ライブラリの定義と同じものだからです。 
-    こうする主な理由は、Coqのグローバルな環境を整理して、例えば、
-    関係する定理を探すのを容易にするためです。*)
-
-Require Export SfLib.
+Require Import Coq.Bool.Bool.
+Require Import Coq.Arith.Arith.
+Require Import Coq.Arith.EqNat.
+Require Import Coq.omega.Omega.
+Require Import Coq.Lists.List.
+Import ListNotations.
+Require Import Maps.
+Require Import SfLib. (* for [admit] *)
 
 (* ####################################################### *)
-(** * Arithmetic and Boolean Expressions *)
+(*  * Arithmetic and Boolean Expressions *)
+(** * 計算式とブール式 *)
 
-(** We'll present Imp in three parts: first a core language of
+(*  We'll present Imp in three parts: first a core language of
     _arithmetic and boolean expressions_, then an extension of these
     expressions with _variables_, and finally a language of _commands_
     including assignment, conditions, sequencing, and loops. *)
+(** 三つの部分に分けて、Impの提示を行います: 最初は、"計算式とブール式"の言語コアを。二番目に、これらに"変数"を追加します。 最後に、代入や条件分岐や連続文やループを含む言語の"コマンド"を追加します。*)
 
 (* ####################################################### *)
 (** ** Syntax *)
 
 Module AExp.
 
-(* These two definitions specify the _abstract syntax_ of
+(*  These two definitions specify the _abstract syntax_ of
     arithmetic and boolean expressions. *)
 (** 次の2つの定義は、算術式とブール式の抽象構文(_abstract syntax_)を定めます。*)
 
@@ -97,14 +86,14 @@ Inductive bexp : Type :=
     1) (AMult (ANum 2) (ANum 3))].  The optional chapter [ImpParser]
     develops a simple implementation of a lexical analyzer and parser
     that can perform this translation.  You do _not_ need to
-    understand that file to understand this one, but if you haven't
+    understand that chapter to understand this one, but if you haven't
     taken a course where these techniques are covered (e.g., a
     compilers course) you may want to skim it. *)
 (** この章では、プログラマが実際に書く具象構文から抽象構文木への変換は省略します。
     例えば、文字列["1+2*3"]をAST(Abstract Syntax Tree, 抽象構文木) 
     [APlus (ANum 1) (AMult (ANum 2) (ANum 3))] にする変換のことです。
     この変換ができる字句解析器と構文解析器をファイル[ImpParser_J.v]で簡単に実装します。
-    このファイル([Imp_J.v])を理解するには[ImpParser_J.v]の理解は必要ではありませんが、
+    この章を理解するには[ImpParser_J.v]の理解は必要ではありませんが、
     もしそれらの技術についてのコース(例えばコンパイラコース)を受講していないならば、
     ざっと見てみるのも良いでしょう。 *)
 
@@ -123,6 +112,7 @@ Inductive bexp : Type :=
         | a <= a
         | not b
         | b and b
+
 *)
 
 (* Compared to the Coq version above...
@@ -132,32 +122,33 @@ Inductive bexp : Type :=
          fact that the addition operation is written [+] and is an
          infix symbol) while leaving other aspects of lexical analysis
          and parsing (like the relative precedence of [+], [-], and
-         [*]) unspecified.  Some additional information -- and human
-         intelligence -- would be required to turn this description
-         into a formal definition (when implementing a compiler, for
-         example).
+         [*], the use of parens to explicitly group subexpressions,
+         etc.) unspecified.  Some additional information (and human
+         intelligence) would be required to turn this description into
+         a formal definition, for example when implementing a
+         compiler.
 
          The Coq version consistently omits all this information and
          concentrates on the abstract syntax only.
 
-       - On the other hand, the BNF version is lighter and
-         easier to read.  Its informality makes it flexible, which is
-         a huge advantage in situations like discussions at the
-         blackboard, where conveying general ideas is more important
-         than getting every detail nailed down precisely.
+       - On the other hand, the BNF version is lighter and easier to
+         read.  Its informality makes it flexible, which is a huge
+         advantage in situations like discussions at the blackboard,
+         where conveying general ideas is more important than getting
+         every detail nailed down precisely.
 
          Indeed, there are dozens of BNF-like notations and people
-         switch freely among them, usually without bothering to say which
-         form of BNF they're using because there is no need to: a
-         rough-and-ready informal understanding is all that's
-         needed. *)
+         switch freely among them, usually without bothering to say
+         which form of BNF they're using because there is no need to:
+         a rough-and-ready informal understanding is all that's
+         important. *)
 (** 上述のCoq版と比較して...
 
        - BNFはより非形式的です。例えば、
          BNFは式の表面的な構文についていくらかの情報を与えています
          (可算は[+]と記述され、それは中置記号であるという事実などです)が、
          字句解析と構文解析の他の面は定めないままになっています([+]、[-]、[*]
-         の相対的優先順位などです)。
+         の相対的優先順位や明示的なカッコによる、部分式のグループ化などです)。
          (例えばコンパイラを実装するときに)この記述を形式的定義にするためには、
          追加の情報、および人間の知性が必要でしょう。
 
@@ -171,7 +162,7 @@ Inductive bexp : Type :=
 
          実際、BNFのような記法は山ほどあり、人は皆、それらの間を自由に行き来しますし、
          通常はそれらのうちのどのBNFを使っているかを気にしません。
-         その必要がないからです。おおざっぱな非形式的な理解だけが必要なのです。 *)
+         その必要がないからです。おおざっぱな非形式的な理解だけが重要なのです。 *)
 
 
 (* It's good to be comfortable with both sorts of notations:
@@ -207,7 +198,7 @@ Fixpoint beval (b : bexp) : bool :=
   | BTrue       => true
   | BFalse      => false
   | BEq a1 a2   => beq_nat (aeval a1) (aeval a2)
-  | BLe a1 a2   => ble_nat (aeval a1) (aeval a2)
+  | BLe a1 a2   => leb (aeval a1) (aeval a2)
   | BNot b1     => negb (beval b1)
   | BAnd b1 b2  => andb (beval b1) (beval b2)
   end.
@@ -216,7 +207,7 @@ Fixpoint beval (b : bexp) : bool :=
 (* ** Optimization *)
 (** ** 最適化(Optimization) *)
 
-(* We haven't defined very much yet, but we can already get
+(*  We haven't defined very much yet, but we can already get
     some mileage out of the definitions.  Suppose we define a function
     that takes an arithmetic expression and slightly simplifies it,
     changing every occurrence of [0+e] (i.e., [(APlus (ANum 0) e])
@@ -239,7 +230,7 @@ Fixpoint optimize_0plus (a:aexp) : aexp :=
       AMult (optimize_0plus e1) (optimize_0plus e2)
   end.
 
-(* To make sure our optimization is doing the right thing we
+(*  To make sure our optimization is doing the right thing we
     can test it on some examples and see if the output looks OK. *)
 (** この最適化が正しいことをすることを確認するために、
     いくつかの例についてテストして出力がよさそうかを見てみることができます。 *)
@@ -251,7 +242,7 @@ Example test_optimize_0plus:
   = APlus (ANum 2) (ANum 1).
 Proof. reflexivity. Qed.
 
-(* But if we want to be sure the optimization is correct --
+(*  But if we want to be sure the optimization is correct --
     i.e., that evaluating an optimized expression gives the same
     result as the original -- we should prove it. *)
 (** しかし、もし最適化が正しいことを確認したいならば、
@@ -262,23 +253,23 @@ Theorem optimize_0plus_sound: forall a,
   aeval (optimize_0plus a) = aeval a.
 Proof.
   intros a. induction a.
-  Case "ANum". reflexivity.
-  Case "APlus". destruct a1.
-    SCase "a1 = ANum n". destruct n.
-      SSCase "n = 0".  simpl. apply IHa2.
-      SSCase "n <> 0". simpl. rewrite IHa2. reflexivity.
-    SCase "a1 = APlus a1_1 a1_2".
+  - (* ANum *) reflexivity.
+  - (* APlus *) destruct a1.
+    + (* a1 = ANum n *) destruct n.
+      * (* n = 0 *)  simpl. apply IHa2.
+      * (* n <> 0 *) simpl. rewrite IHa2. reflexivity.
+    + (* a1 = APlus a1_1 a1_2 *)
       simpl. simpl in IHa1. rewrite IHa1.
       rewrite IHa2. reflexivity.
-    SCase "a1 = AMinus a1_1 a1_2".
+    + (* a1 = AMinus a1_1 a1_2 *)
       simpl. simpl in IHa1. rewrite IHa1.
       rewrite IHa2. reflexivity.
-    SCase "a1 = AMult a1_1 a1_2".
+    + (* a1 = AMult a1_1 a1_2 *)
       simpl. simpl in IHa1. rewrite IHa1.
       rewrite IHa2. reflexivity.
-  Case "AMinus".
+  - (* AMinus *)
     simpl. rewrite IHa1. rewrite IHa2. reflexivity.
-  Case "AMult".
+  - (* AMult *)
     simpl. rewrite IHa1. rewrite IHa2. reflexivity.  Qed.
 
 (* ####################################################### *)
@@ -382,41 +373,46 @@ Qed.
 (* Using [try] in a completely manual proof is a bit silly, but
     we'll see below that [try] is very useful for doing automated
     proofs in conjunction with the [;] tactical. *)
-(** [try]タクティックを手動の証明で使用することは少し馬鹿げていると思われるかもしれまんが、
+(** [try]タクティックを手動の証明で使用する現実的な理由は何もありませんが、
 こみいった自動化された証明において、[;]と同時に使用することで非常に便利になります *)
 (* ####################################################### *)
-(* *** The [;] Tactical (Simple Form) *)
+(*  *** The [;] Tactical (Simple Form) *)
 (** *** [;]タクティカル(単純な形式) *)
 
-(* In its most commonly used form, the [;] tactical takes two tactics
-    as argument: [T;T'] first performs the tactic [T] and then
-    performs the tactic [T'] on _each subgoal_ generated by [T]. *)
-(** [;]が最も使用されるのは、[T;T']ように、二つのタクティックを引数にとるやりかたです。最初にタクティック[T]が実行され、
-次にタクティック[T']が[T]によって生成された、それぞれのサブゴールにおいて実行されます。*)
-(* For example, consider the following trivial lemma: *)
+(*  In its most common form, the [;] tactical takes two tactics as
+    arguments.  The compound tactic [T;T'] first performs [T] and then
+    performs [T'] on _each subgoal_ generated by [T]. *)
+(** [;]が最も使用されるのは、[T;T']ように、二つのタクティックを引数にとるやりかたです。合成されたタクティック[T;T']は、最初に[T]が実行され、
+次に[T']が[T]によって生成された、それぞれのサブゴールにおいて実行されます。*)
+
+(*  For example, consider the following trivial lemma: *)
 (** 例として、次のちょっとした補題について考えてみましょう: *)
 
-Lemma foo : forall n, ble_nat 0 n = true.
+Lemma foo : forall n, leb 0 n = true.
 Proof.
   intros.
   destruct n.
-    (* Leaves two subgoals, which are discharged identically...  *)
-    Case "n=0". simpl. reflexivity.
-    Case "n=Sn'". simpl. reflexivity.
+    (* Leaves two subgoals, which are discharged 
+       identically...  *)
+    - (* n=0 *) simpl. reflexivity.
+    - (* n=Sn' *) simpl. reflexivity.
 Qed.
 
 (* We can simplify this proof using the [;] tactical: *)
 (** [;] タクティカルを使用することで証明がシンプルになります。: *)
 
-Lemma foo' : forall n, ble_nat 0 n = true.
+Lemma foo' : forall n, leb 0 n = true.
 Proof.
   intros.
-  destruct n; (* [destruct] the current goal *)
-  simpl; (* then [simpl] each resulting subgoal *)
-  reflexivity. (* and do [reflexivity] on each resulting subgoal *)
+  (* 現在のゴールを[destruct] *)
+  destruct n; 
+  (* それから それぞれのサブゴールで[simpl]を実行 *)
+  simpl; 
+  (* そしてそれぞれのサブゴールの結果に対して[reflexivity]を実行 *)
+  reflexivity. 
 Qed.
 
-(* Using [try] and [;] together, we can get rid of the repetition in
+(*  Using [try] and [;] together, we can get rid of the repetition in
     the proof that was bothering us a little while ago. *)
 (** [try]と[;]の両方を使うと、
     ちょっと前に悩まされた証明の繰り返しを取り除くことができます。 *)
@@ -429,8 +425,8 @@ Proof.
     (* Most cases follow directly by the IH *)
     try (simpl; rewrite IHa1; rewrite IHa2; reflexivity).
   (* The remaining cases -- ANum and APlus -- are different *)
-  Case "ANum". reflexivity.
-  Case "APlus".
+  - (* ANum *) reflexivity.
+  - (* APlus *)
     destruct a1;
       (* Again, most cases follow directly by the IH *)
       try (simpl; simpl in IHa1; rewrite IHa1;
@@ -439,7 +435,7 @@ Proof.
        is when [e1 = ANum n]. In this case, we have to destruct
        [n] (to see whether the optimization applies) and rewrite
        with the induction hypothesis. *)
-    SCase "a1 = ANum n". destruct n;
+    + (* a1 = ANum n *) destruct n;
       simpl; rewrite IHa2; reflexivity.   Qed.
 
 (* Coq experts often use this "[...; try... ]" idiom after a tactic
@@ -534,27 +530,31 @@ Proof.
     (* ... or are immediate by definition *)
     try reflexivity.
   (* The interesting case is when a = APlus a1 a2. *)
-  Case "APlus".
+  - (* APlus *)
     destruct a1; try (simpl; simpl in IHa1; rewrite IHa1;
                       rewrite IHa2; reflexivity).
-    SCase "a1 = ANum n". destruct n;
+    + (* a1 = ANum n *) destruct n;
       simpl; rewrite IHa2; reflexivity. Qed.
 
 (* ####################################################### *)
-(* *** The [;] Tactical (General Form) *)
+(*  *** The [;] Tactical (General Form) *)
 (** *** [;] タクティカル (一般的な形式) *)
 
-(* The [;] tactical has a more general than the simple [T;T'] we've
-    seen above, which is sometimes also useful.  If [T], [T1], ...,
-    [Tn] are tactics, then
+(*  The [;] tactical also has a more general form than the simple
+    [T;T'] we've seen above.  If [T], [T1], ..., [Tn] are tactics,
+    then
+
       T; [T1 | T2 | ... | Tn]
+
    is a tactic that first performs [T] and then performs [T1] on the
    first subgoal generated by [T], performs [T2] on the second
    subgoal, etc.
 
    So [T;T'] is just special notation for the case when all of the
-   [Ti]'s are the same tactic; i.e. [T;T'] is just a shorthand for:
+   [Ti]'s are the same tactic -- i.e., [T;T'] is shorthand for:
+
       T; [T' | T' | ... | T']
+
 *)
 (** 上記で見た、単純な、[T;T']よりも一般的に[;]を使うことが出来、しぱしば有用です。[T],[T1],...,[Tn]がタクティカルならば、
     T; [T1| T2 | ... | Tn]
@@ -562,35 +562,112 @@ Proof.
    [T]によって生成された最初のサブゴールに[T1]を行ない、
    二番目のサブゴールに[T2]を行ない、... という処理をします。 
    すべての[Ti]が同じタクティック[T']であるという特別な場合、
+
       T; [T' | T' | ... | T']
+
    と書く代わりに [T;T'] と書くだけで済ますことができます。*)
 
 (* ####################################################### *)
-(* ** Defining New Tactic Notations *)
+(* *** The [repeat] Tactical *)
+(** *** [repeat] タクティカル *)
+
+(*  The [repeat] tactical takes another tactic and keeps applying this
+    tactic until it fails. Here is an example showing that [10] is in
+    a long list using repeat. *)
+(** [repeat]タクティカルは、別のタクティックを引数として取り、そのタクティックが失敗するまで適用を続けます。
+以下は、repeatを使用した[10]がある長いリストの中にあることを示す例です。*)
+
+Theorem In10 : In 10 [1;2;3;4;5;6;7;8;9;10].
+Proof.
+  repeat (try (left; reflexivity); right). 
+Qed.
+(* Print In10. *)
+
+(*  The [repeat T] tactic never fails: if the tactic [T] doesn't apply
+    to the original goal, then repeat still succeeds without changing
+    the original goal (i.e., it repeats zero times). *)
+(** [repeat T]タクティックは決して失敗しません。もし、タクティック[T]が現在のゴールに適用できない場合、ゴールを変更することなく、成功するまで繰り返します。(つまり0回繰り返します。*)
+
+Theorem In10' : In 10 [1;2;3;4;5;6;7;8;9;10].
+Proof.
+  repeat (left; reflexivity). 
+  repeat (right; try (left; reflexivity)). 
+Qed.
+
+(*  The [repeat T] tactic also does not have any bound on the
+    number of times it applies [T].  If [T] is a tactic that always
+    succeeds, then repeat [T] will loop forever (e.g., [repeat simpl]
+    loops forever, since [simpl] always succeeds).  While Coq's term
+    language is guaranteed to terminate, Coq's tactic language is
+    not! *)
+(** [repeat T]タクティックは、[T]を適用する回数の限界値について関知しません。
+    もし、[T]が常に成功する場合、[T]を永久に繰り返します。(例えば、[repeat simpl]は
+    [simpl]が常に成功するため、無限ループします。) Coqは自身の言語については、終了を保証していますが、
+    Coqのタクティック言語については、そうではないのです。*)
+
+(*  **** Exercise: 3 stars (optimize_0plus_b) *)
+(** **** 練習問題: ★★★ (optimize_0plus_b) *)
+(*  Since the [optimize_0plus] tranformation doesn't change the value
+    of [aexp]s, we should be able to apply it to all the [aexp]s that
+    appear in a [bexp] without changing the [bexp]'s value.  Write a
+    function which performs that transformation on [bexp]s, and prove
+    it is sound.  Use the tacticals we've just seen to make the proof
+    as elegant as possible. *)
+(** [optimize_0plus]の変換が[aexp]の値を変えないことから、
+    [bexp]の値を変えずに、[bexp]に現れる[aexp]をすべて変換するために
+    [optimize_0plus]が適用できるべきでしょう。
+    [bexp]についてこの変換をする関数を記述しなさい。そして、
+    それが健全であることを証明しなさい。
+    ここまで見てきたタクティカルを使って証明を可能な限りエレガントにしなさい。*)
+
+Fixpoint optimize_0plus_b (b : bexp) : bexp :=
+  (* FILL IN HERE *) admit.
+
+Theorem optimize_0plus_b_sound : forall b,
+  beval (optimize_0plus_b b) = beval b.
+Proof.
+  (* FILL IN HERE *) Admitted.
+(** [] *)
+
+(*  **** Exercise: 4 stars, optional (optimizer) *)
+(** **** 練習問題: ★★★★, optional (optimizer) *)
+(*  _Design exercise_: The optimization implemented by our
+    [optimize_0plus] function is only one of many possible
+    optimizations on arithmetic and boolean expressions.  Write a more
+    sophisticated optimizer and prove it correct.  *)
+(** 設計練習: 定義した[optimize_0plus]関数で実装された最適化は、
+    算術式やブール式に対して実行可能な、いろいろな最適化の単なる1つに過ぎません。
+    より洗練された最適化関数を記述し、その正しさを証明しなさい。
+
+(* FILL IN HERE *)
+*)
+(** [] *)
+
+(* ####################################################### *)
+(*  ** Defining New Tactic Notations *)
 (** ** 新しいタクティック記法を定義する *)
 
-(* Coq also provides several ways of "programming" tactic scripts.
+(*  Coq also provides several ways of "programming" tactic scripts.
 
-      - The [Tactic Notation] idiom illustrated below gives a handy
-        way to define "shorthand tactics" that bundle several tactics
-        into a single command.
+    - The [Tactic Notation] idiom illustrated below gives a handy way to
+      define "shorthand tactics" that bundle several tactics into a
+      single command.
 
-      - For more sophisticated programming, Coq offers a small
-        built-in programming language called [Ltac] with primitives
-        that can examine and modify the proof state.  The details are
-        a bit too complicated to get into here (and it is generally
-        agreed that [Ltac] is not the most beautiful part of Coq's
-        design!), but they can be found in the reference manual, and
-        there are many examples of [Ltac] definitions in the Coq
-        standard library that you can use as examples.
+    - For more sophisticated programming, Coq offers a small built-in
+      programming language called [Ltac] with primitives that can
+      examine and modify the proof state.  The details are a bit too
+      complicated to get into here (and it is generally agreed that
+      [Ltac] is not the most beautiful part of Coq's design!), but they
+      can be found in the reference manual and other books on Coq, and
+      there are many examples of [Ltac] definitions in the Coq standard
+      library that you can use as examples.
 
-      - There is also an OCaml API, which can be used to build tactics
-        that access Coq's internal structures at a lower level, but
-        this is seldom worth the trouble for ordinary Coq users.
+    - There is also an OCaml API, which can be used to build tactics
+      that access Coq's internal structures at a lower level, but this
+      is seldom worth the trouble for ordinary Coq users.
 
-The [Tactic Notation] mechanism is the easiest to come to grips with,
-and it offers plenty of power for many purposes.  Here's an example.
-*)
+    The [Tactic Notation] mechanism is the easiest to come to grips with,
+    and it offers plenty of power for many purposes.  Here's an example. *)
 (** Coqはまた、タクティックスクリプトを「プログラミングする」いろいろな方法も提供します。
 
       - [Tactic Notation] コマンドは、「略記法タクティック」("shorthand tactics")
@@ -617,142 +694,16 @@ Tactic Notation "simpl_and_try" tactic(c) :=
   simpl;
   try c.
 
-(* This defines a new tactical called [simpl_and_try] which
-    takes one tactic [c] as an argument, and is defined to be
-    equivalent to the tactic [simpl; try c].  For example, writing
-    "[simpl_and_try reflexivity.]" in a proof would be the same as
-    writing "[simpl; try reflexivity.]" *)
+(*  This defines a new tactical called [simpl_and_try] that takes one
+    tactic [c] as an argument and is defined to be equivalent to the
+    tactic [simpl; try c].  For example, writing "[simpl_and_try
+    reflexivity.]" in a proof would be the same as writing "[simpl;
+    try reflexivity.]" *)
 (** これは1つのタクティック[c]を引数としてとる[simpl_and_try]
     という新しいタクティカルを定義しています。
     そして、タクティック [simpl; try c] と同値なものとして定義されます。
     例えば、証明内で"[simpl_and_try reflexivity.]"と書くことは
     "[simpl; try reflexivity.]"と書くことと同じでしょう。 *)
-
-(* The next subsection gives a more sophisticated use of this
-    feature... *)
-(** 次のサブセクションでは、この機構のより洗練された使い方を見ます... *)
-
-(* ####################################################### *)
-(* *** Bulletproofing Case Analyses *)
-(** *** 場合分けを万全にする *)
-
-(** Being able to deal with most of the cases of an [induction]
-    or [destruct] all at the same time is very convenient, but it can
-    also be a little confusing.  One problem that often comes up is
-    that _maintaining_ proofs written in this style can be difficult.
-    For example, suppose that, later, we extended the definition of
-    [aexp] with another constructor that also required a special
-    argument.  The above proof might break because Coq generated the
-    subgoals for this constructor before the one for [APlus], so that,
-    at the point when we start working on the [APlus] case, Coq is
-    actually expecting the argument for a completely different
-    constructor.  What we'd like is to get a sensible error message
-    saying "I was expecting the [AFoo] case at this point, but the
-    proof script is talking about [APlus]."  Here's a nice trick (due
-    to Aaron Bohannon) that smoothly achieves this. *)
-(** [induction]や[destruct]で、ほとんどの場合を一度に扱えるのはとても便利ですが、
-    またちょっと混乱もします。よく起こる問題は、
-    このスタイルで記述された証明をメンテナンスすることが難しいということです。
-    例えば、後で、[aexp]の定義を拡張して、
-    やはり特別な引数をとるコンストラクタを追加したとします。
-    このとき上述の証明は成立しなくなっているでしょう。
-    なぜなら、
-    Coqは[APlus]についてのサブゴールの前にこのコンストラクタに対応するサブゴールを生成し、
-    その結果、[APlus]の場合に取りかかる時には、
-    Coqは実際にはまったく別のコンストラクタを待っていることになるからです。
-    ここで欲しいのは、「この場所で[AFoo]の場合を期待していましたが、
-    証明スクリプトは[APlus]について話しています。」という賢いエラーメッセージです。
-    以下は、これを難なく可能にするちょっとしたトリックです。 *)
-
-Tactic Notation "aexp_cases" tactic(first) ident(c) :=
-  first;
-  [ Case_aux c "ANum" | Case_aux c "APlus"
-  | Case_aux c "AMinus" | Case_aux c "AMult" ].
-
-(* ([Case_aux] implements the common functionality of [Case],
-    [SCase], [SSCase], etc.  For example, [Case "foo"] is defined as
-    [Case_aux Case "foo".) *)
-(** ([Case_aux]は[Case]、[SCase]、[SSCase]等の共通機能を実装します。
-    例えば、[Case "foo"]は [Case_aux Case "foo"] と定義されます。) *)
-
-(* For example, if [a] is a variable of type [aexp], then doing
-      aexp_cases (induction a) Case
-    will perform an induction on [a] (the same as if we had just typed
-    [induction a]) and _also_ add a [Case] tag to each subgoal
-    generated by the [induction], labeling which constructor it comes
-    from.  For example, here is yet another proof of
-    [optimize_0plus_sound], using [aexp_cases]: *)
-(** 例えば、[a]が型[aexp]の変数のとき、
-      aexp_cases (induction e) Case
-    と書くと[a]についての帰納法を実行し(単に [induction e] と書いたのと同じです)、
-    そして、「その上に」、[induction]によって生成されたそれぞれのサブゴールに[Case]
-    タグを付加します。このタグは、そのサブゴールがどのコンストラクタから来たかのラベルです。
-    例えば、[aexp_cases]を使った、[optimize_0plus_sound]のさらに別証です: *)
-
-tsi
-  intros a.
-  aexp_cases (induction a) Case;
-    try (simpl; rewrite IHa1; rewrite IHa2; reflexivity);
-    try reflexivity.
-  (* At this point, there is already an ["APlus"] case name
-     in the context.  The [Case "APlus"] here in the proof
-     text has the effect of a sanity check: if the "Case"
-     string in the context is anything _other_ than ["APlus"]
-     (for example, because we added a clause to the definition
-     of [aexp] and forgot to change the proof) we'll get a
-     helpful error at this point telling us that this is now
-     the wrong case. *)
-  (* この時点で、すでに["APlus"]の名前はコンテキストに導入されています。
-  [Case "Aplus"]のテキストは証明のこの時点で健全性のチェックの効果を持ちます。
-  ：もし、コンテキスト中の"Case"文字列が["APlus"]ではない他のものである場合、(例えば、[aexp]に後から追加されていたにも係らず、証明の変更を忘れていたなど)ここで場合分けが間違っていることに気が付くことが出来ます。*)
-  Case "APlus".
-    aexp_cases (destruct a1) SCase;
-      try (simpl; simpl in IHa1;
-           rewrite IHa1; rewrite IHa2; reflexivity).
-    SCase "ANum". destruct n;
-      simpl; rewrite IHa2; reflexivity.  Qed.
-
-(*  **** Exercise: 3 stars (optimize_0plus_b) *)
-(*  Since the [optimize_0plus] tranformation doesn't change the value
-    of [aexp]s, we should be able to apply it to all the [aexp]s that
-    appear in a [bexp] without changing the [bexp]'s value.  Write a
-    function which performs that transformation on [bexp]s, and prove
-    it is sound.  Use the tacticals we've just seen to make the proof
-    as elegant as possible. *)
-(** **** 練習問題: ★★★ (optimize_0plus_b) *)
-(** [optimize_0plus]の変換が[aexp]の値を変えないことから、
-    [bexp]の値を変えずに、[bexp]に現れる[aexp]をすべて変換するために
-    [optimize_0plus]が適用できるべきでしょう。
-    [bexp]についてこの変換をする関数を記述しなさい。そして、
-    それが健全であることを証明しなさい。
-    ここまで見てきたタクティカルを使って証明を可能な限りエレガントにしなさい。*)
-
-Fixpoint optimize_0plus_b (b : bexp) : bexp :=
-  (* FILL IN HERE *) admit.
-
-
-Theorem optimize_0plus_b_sound : forall b,
-  beval (optimize_0plus_b b) = beval b.
-Proof.
-  (* FILL IN HERE *) Admitted.
-(** [] *)
-
-(*  **** Exercise: 4 stars, optional (optimizer) *)
-(*  _Design exercise_: The optimization implemented by our
-    [optimize_0plus] function is only one of many imaginable
-    optimizations on arithmetic and boolean expressions.  Write a more
-    sophisticated optimizer and prove it correct.
-
-(* FILL IN HERE *)
-*)
-(** **** 練習問題: ★★★★, optional (optimizer) *)
-(** 設計練習: 定義した[optimize_0plus]関数で実装された最適化は、
-    算術式やブール式に対して考えられるいろいろな最適化の単なる1つに過ぎません。
-    より洗練された最適化関数を記述し、その正しさを証明しなさい。
-
-(* FILL IN HERE *)
-*)
-(** [] *)
 
 (* ####################################################### *)
 (* ** The [omega] Tactic *)
@@ -760,7 +711,7 @@ Proof.
 
 (* The [omega] tactic implements a decision procedure for a subset of
     first-order logic called _Presburger arithmetic_.  It is based on
-    the Omega algorithm invented in 1992 by William Pugh.
+    the Omega algorithm invented in 1991 by William Pugh [Pugh 1991].
 
     If the goal is a universally quantified formula made out of
 
@@ -798,13 +749,14 @@ Proof.
   intros. omega.
 Qed.
 
-(** Liebniz wrote, "It is unworthy of excellent men to lose
+(*  Leibniz wrote, "It is unworthy of excellent men to lose
     hours like slaves in the labor of calculation which could be
     relegated to anyone else if machines were used."  We recommend
-    using the omega tactic whenever possible. *)
+    that excellent people of all genders use the omega tactic whenever
+    possible. *)
 (** "優れた人間が奴隷に格下げになるような機械でも出来るような誰でも出来る計算に従事して時間を無駄にすることほど勿体ないことはない。"とライプニッツは書いています。*)
 (* ####################################################### *)
-(* ** A Few More Handy Tactics *)
+(*  ** A Few More Handy Tactics *)
 (** ** 便利なタクティックをさらにいくつか *)
 
 (** Finally, here are some miscellaneous tactics that you may find
@@ -835,8 +787,9 @@ Qed.
      - [constructor]: Try to find a constructor [c] (from some
        [Inductive] definition in the current environment) that can be
        applied to solve the current goal.  If one is found, behave
-       like [apply c]. *)
+       like [apply c]. 
 
+    We'll see many examples of these in the proofs below. *)
 (** 最後に、役に立ちそうないろいろなタクティックをいくつか紹介します。
 
      - [clear H]: 仮定[H]をコンテキストから消去します。
@@ -859,21 +812,19 @@ Qed.
 
      - [constructor]: 現在のゴールを解くのに使えるコンストラクタ[c]を
        (現在の環境の[Inductive]による定義から)探そうとします。
-       発見されたときは [apply c] と同様に振る舞います。 *)
+       発見されたときは [apply c] と同様に振る舞います。
 
-(* We'll see many examples of these in the proofs below. *)
-(** 以降の証明でこれらのたくさんの例を見るでしょう。 *)
+       以降の証明でこれらのたくさんの例を見るでしょう。 *)
 
 (* ####################################################### *)
 (* * Evaluation as a Relation *)
 (** * 関係としての評価 *)
 
 (* We have presented [aeval] and [beval] as functions defined by
-    [Fixpoints].  Another way to think about evaluation -- one that we
+    [Fixpoint]s.  Another way to think about evaluation -- one that we
     will see is often more flexible -- is as a _relation_ between
     expressions and their values.  This leads naturally to [Inductive]
-    definitions like the following one for arithmetic
-    expressions... *)
+    definitions like the following one for arithmetic expressions... *)
 (** [aeval]と[beval]を[Fixpoints]によって定義された関数として示しました。
     評価について考える別の方法は、それを式と値との間の関係(_relation_)と見ることです。
 
@@ -901,50 +852,53 @@ Inductive aevalR : aexp -> nat -> Prop :=
 
 (** As is often the case with relations, we'll find it
     convenient to define infix notation for [aevalR].  We'll write [e
-    || n] to mean that arithmetic expression [e] evaluates to value
+    \\ n] to mean that arithmetic expression [e] evaluates to value
     [n].  (This notation is one place where the limitation to ASCII
     symbols becomes a little bothersome.  The standard notation for
     the evaluation relation is a double down-arrow.  We'll typeset it
-    like this in the HTML version of the notes and use a double
-    vertical bar as the closest approximation in [.v] files.)  *)
+    like this in the HTML version of the notes and use a double slash
+    as the closest approximation in [.v] files.)  *)
 (** 関係についてよく行うように、[aevalR]の中置記法を定義するのが便利です。
-    算術式[e]が値[n]に評価されることを [e || n] と書きます。
+    算術式[e]が値[n]に評価されることを [e \\ n] と書きます。
     (この記法は煩わしいascii記号の限界の1つです。評価関係の標準記法は二重の下向き矢印です。
     HTML版ではそのようにタイプセットしますが、ascii の
     .v ファイルでは可能な近似として縦棒二本を使います。) *)
 
-Notation "e '||' n" := (aevalR e n) : type_scope.
+Notation "e '\\' n"
+         := (aevalR e n) 
+            (at level 50, left associativity)
+         : type_scope.
 
 End aevalR_first_try.
 
 (* In fact, Coq provides a way to use this notation in the definition
     of [aevalR] itself.  This avoids situations where we're working on
-    a proof involving statements in the form [e || n] but we have to
+    a proof involving statements in the form [e \\ n] but we have to
     refer back to a definition written using the form [aevalR e n].
 
     We do this by first "reserving" the notation, then giving the
     definition together with a declaration of what the notation
     means. *)
 (** 実際は、Coqでは[aevalR]自身の定義中でこの記法を使うことができます。
-    これにより、[e || n] の形の主張を含む証明で、[aevalR e n] 
+    これにより、[e \\ n] の形の主張を含む証明で、[aevalR e n] 
     という形の定義に戻らなければならない状況にならずに済みます。
 
     このためには、最初に記法を「予約」し、
     それから定義と、記法が何を意味するかの宣言とを一緒に行います。*)
 
-Reserved Notation "e '||' n" (at level 50, left associativity).
+Reserved Notation "e '\\' n" (at level 50, left associativity).
 
 Inductive aevalR : aexp -> nat -> Prop :=
   | E_ANum : forall (n:nat),
-      (ANum n) || n
+      (ANum n) \\ n
   | E_APlus : forall (e1 e2: aexp) (n1 n2 : nat),
-      (e1 || n1) -> (e2 || n2) -> (APlus e1 e2) || (n1 + n2)
+      (e1 \\ n1) -> (e2 \\ n2) -> (APlus e1 e2) \\ (n1 + n2)
   | E_AMinus : forall (e1 e2: aexp) (n1 n2 : nat),
-      (e1 || n1) -> (e2 || n2) -> (AMinus e1 e2) || (n1 - n2)
+      (e1 \\ n1) -> (e2 \\ n2) -> (AMinus e1 e2) \\ (n1 - n2)
   | E_AMult :  forall (e1 e2: aexp) (n1 n2 : nat),
-      (e1 || n1) -> (e2 || n2) -> (AMult e1 e2) || (n1 * n2)
+      (e1 \\ n1) -> (e2 \\ n2) -> (AMult e1 e2) \\ (n1 * n2)
 
-  where "e '||' n" := (aevalR e n) : type_scope.
+  where "e '\\' n" := (aevalR e n) : type_scope.
 
 Tactic Notation "aevalR_cases" tactic(first) ident(c) :=
   first;
@@ -966,16 +920,19 @@ Tactic Notation "aevalR_cases" tactic(first) ident(c) :=
     推論規則は、横線の上の前提から、横線の下の結論を導出できることを述べます。
 	( すでに、Propの章で見ていると思いますが。) *)
 
-(* For example, the constructor [E_APlus]...
+(*  For example, the constructor [E_APlus]...
       | E_APlus : forall (e1 e2: aexp) (n1 n2: nat),
           aevalR e1 n1 ->
           aevalR e2 n2 ->
           aevalR (APlus e1 e2) (n1 + n2)
+
     ...would be written like this as an inference rule:
-                               e1 || n1
-                               e2 || n2
+
+                               e1 \\ n1
+                               e2 \\ n2
                          --------------------                         (E_APlus)
-                         APlus e1 e2 || n1+n2
+                         APlus e1 e2 \\ n1+n2
+
 *)
 (** 例えば、コンストラクタ[E_APlus]...
       | E_APlus : forall (e1 e2: aexp) (n1 n2: nat),
@@ -983,145 +940,122 @@ Tactic Notation "aevalR_cases" tactic(first) ident(c) :=
           aevalR e2 n2 ->
           aevalR (APlus e1 e2) (n1 + n2)
     ...は推論規則として次のように書けるでしょう:
-                               e1 || n1
-                               e2 || n2
+                               e1 \\ n1
+                               e2 \\ n2
                          --------------------                         (E_APlus)
-                         APlus e1 e2 || n1+n2
+                         APlus e1 e2 \\ n1+n2
 *)
-(* Formally, there is nothing very deep about inference rules:
-    they are just implications.  You can read the rule name on the
-    right as the name of the constructor and read each of the
-    linebreaks between the premises above the line and the line itself
-    as [->].  All the variables mentioned in the rule ([e1], [n1],
-    etc.) are implicitly bound by universal quantifiers at the
-    beginning. (Such variables are often called _metavariables_ to
-    distinguish them from the variables of the language we are
-    defining.  At the moment, our arithmetic expressions don't include
-    variables, but we'll soon be adding them.)  The whole collection
-    of rules is understood as being wrapped in an [Inductive]
-    declaration (informally, this is either elided or else indicated
-    by saying something like "Let [aevalR] be the smallest relation
-    closed under the following rules..."). *)
+
+(*  Formally, there is nothing deep about inference rules: they
+    are just implications.  You can read the rule name on the right as
+    the name of the constructor and read each of the linebreaks
+    between the premises above the line and the line itself as [->].
+    All the variables mentioned in the rule ([e1], [n1], etc.) are
+    implicitly bound by universal quantifiers at the beginning. (Such
+    variables are often called _metavariables_ to distinguish them
+    from the variables of the language we are defining.  At the
+    moment, our arithmetic expressions don't include variables, but
+    we'll soon be adding them.)  The whole collection of rules is
+    understood as being wrapped in an [Inductive] declaration.  In
+    informal prose, this is either elided or else indicated by saying
+    something like "Let [aevalR] be the smallest relation closed under
+    the following rules...". *)
 (** 形式的には、推論規則について何も深いものはありません。単なる含意です。
     右に書かれた規則名はコンストラクタで、
     横線より上の前提の間の各改行と横線自体は[->]と読むことができます。
     規則で言及されるすべての変数([e1]、[n1]等)
     は暗黙のうちに冒頭で全称限量子に束縛されています。
     規則の集合全体は[Inductive]宣言で囲われていると理解されます
-    (これは完全に暗黙のまま置かれるか、非形式的に
+    これは完全に暗黙のまま置かれるか、非形式的に
     「[aevalR]は以下の規則について閉じた最小の関係とします...」
-    などと述べられるかします)。 *)
-(* For example, [||] is the smallest relation closed under these
-    rules:
+    などと述べられるかします。 *)
+
+(*  For example, [\\] is the smallest relation closed under these
+    rules: *)
+(** 例えば、[\\]は以下の規則について閉じた最小の関係です:
+
                              -----------                               (E_ANum)
-                             ANum n || n
+                             ANum n \\ n
 
-                               e1 || n1
-                               e2 || n2
+                               e1 \\ n1
+                               e2 \\ n2
                          --------------------                         (E_APlus)
-                         APlus e1 e2 || n1+n2
+                         APlus e1 e2 \\ n1+n2
 
-                               e1 || n1
-                               e2 || n2
+                               e1 \\ n1
+                               e2 \\ n2
                         ---------------------                        (E_AMinus)
-                        AMinus e1 e2 || n1-n2
+                        AMinus e1 e2 \\ n1-n2
 
-                               e1 || n1
-                               e2 || n2
+                               e1 \\ n1
+                               e2 \\ n2
                          --------------------                         (E_AMult)
-                         AMult e1 e2 || n1*n2
-*)
-(** 例えば、[||]は以下の規則について閉じた最小の関係です:
-                             -----------                               (E_ANum)
-                             ANum n || n
+                         AMult e1 e2 \\ n1*n2
 
-                               e1 || n1
-                               e2 || n2
-                         --------------------                         (E_APlus)
-                         APlus e1 e2 || n1+n2
-
-                               e1 || n1
-                               e2 || n2
-                        ---------------------                        (E_AMinus)
-                        AMinus e1 e2 || n1-n2
-
-                               e1 || n1
-                               e2 || n2
-                         --------------------                         (E_AMult)
-                         AMult e1 e2 || n1*n2
 *)
 
 (* ####################################################### *)
-(* ** Equivalence of the Definitions *)
+(*  ** Equivalence of the Definitions *)
 (** ** 等価性の定義 *)
-(* It is straightforward to prove that the relational and functional
-    definitions of evaluation agree on all possible arithmetic
-    expressions... *)
-(** 関係による定義と、関数による定義とが、評価が有り得る全ての算術式において一致することの直接的な証明です。*)
+(*  It is straightforward to prove that the relational and functional
+    definitions of evaluation agree, for all arithmetic expressions... *)
+(** 関係による定義と、関数による定義とが、全ての算術式において評価が一致することの直接的な証明です。*)
+
 Theorem aeval_iff_aevalR : forall a n,
-  (a || n) <-> aeval a = n.
+  (a \\ n) <-> aeval a = n.
 Proof.
  split.
- Case "->".
+ - (* -> *)
    intros H.
-   aevalR_cases (induction H) SCase; simpl.
-   SCase "E_ANum".
+   induction H; simpl.
+   + (* E_ANum *)
      reflexivity.
-   SCase "E_APlus".
+   + (* E_APlus *)
      rewrite IHaevalR1.  rewrite IHaevalR2.  reflexivity.
-   SCase "E_AMinus".
+   + (* E_AMinus *)
      rewrite IHaevalR1.  rewrite IHaevalR2.  reflexivity.
-   SCase "E_AMult".
+   + (* E_AMult *)
      rewrite IHaevalR1.  rewrite IHaevalR2.  reflexivity.
- Case "<-".
+ - (* <- *)
    generalize dependent n.
-   aexp_cases (induction a) SCase;
+   induction a;
       simpl; intros; subst.
-   SCase "ANum".
+   + (* ANum *)
      apply E_ANum.
-   SCase "APlus".
+   + (* APlus *)
      apply E_APlus.
       apply IHa1. reflexivity.
       apply IHa2. reflexivity.
-   SCase "AMinus".
+   + (* AMinus *)
      apply E_AMinus.
       apply IHa1. reflexivity.
       apply IHa2. reflexivity.
-   SCase "AMult".
+   + (* AMult *)
      apply E_AMult.
       apply IHa1. reflexivity.
       apply IHa2. reflexivity.
 Qed.
 
-(* Note: if you're reading the HTML file, you'll see an empty square box instead
-of a proof for this theorem.  
-You can click on this box to "unfold" the text to see the proof.
-Click on the unfolded to text to "fold" it back up to a box. We'll be using
-this style frequently from now on to help keep the HTML easier to read.
-The full proofs always appear in the .v files. *)
-(** 注意： もし、HTMLファイルを読んでいるならば、この定理の証明の代わりに白抜きの四角形が表示されているかもしれません。
-その場合は、その四角形をクリックすることで、折り畳まれた証明を"unfold"して見てください。展開された証明はクリックすると折り畳まれます。
-これから、HTMLの読み易さのためにしばしばこの形式を用います。完全な証明は常に、.vファイルにあります *)
-
-(* We can make the proof quite a bit shorter by making more
+(*  We can make the proof quite a bit shorter by making more
     use of tacticals... *)
 (** タクティカルを使用することで、証明はもっと全然短かくすることができます。*) 
+
 Theorem aeval_iff_aevalR' : forall a n,
-  (a || n) <-> aeval a = n.
+  (a \\ n) <-> aeval a = n.
 Proof.
   (* WORKED IN CLASS *)
   split.
-  Case "->".
+  - (* -> *)
     intros H; induction H; subst; reflexivity.
-  Case "<-".
+  - (* <- *)
     generalize dependent n.
     induction a; simpl; intros; subst; constructor;
        try apply IHa1; try apply IHa2; reflexivity.
 Qed.
 
-(* **** Exercise: 3 stars  (bevalR) *)
+(*  **** Exercise: 3 stars  (bevalR) *)
 (** **** 練習問題: ★★★  (bevalR) *)
-(* Write a relation [bevalR] in the same style as
+(*  Write a relation [bevalR] in the same style as
     [aevalR], and prove that it is equivalent to [beval].*)
 (** 関係[bevalR]を[aevalR]と同じ形式で書きなさい。そしてそれが、[beval]と等価であることを証明しなさい。 *)
 (* 
@@ -1129,6 +1063,7 @@ Inductive bevalR:
 (* FILL IN HERE *)
 *)
 (** [] *)
+
 End AExp.
 
 (* ####################################################### *)
@@ -1157,7 +1092,7 @@ End AExp.
 
 Module aevalR_division.
 
-(* For example, suppose that we wanted to extend the arithmetic
+(*  For example, suppose that we wanted to extend the arithmetic
     operations by considering also a division operation:*)
 (** たとえば、算術の操作を割り算を加えて拡張しようと思ったとしましょう *)
 
@@ -1168,34 +1103,48 @@ Inductive aexp : Type :=
   | AMult : aexp -> aexp -> aexp
   | ADiv : aexp -> aexp -> aexp.   (* <--- new *)
 
-(* Extending the definition of [aeval] to handle this new operation
+(*  Extending the definition of [aeval] to handle this new operation
     would not be straightforward (what should we return as the result
     of [ADiv (ANum 5) (ANum 0)]?).  But extending [aevalR] is
     straightforward. *)
 (** この新しい操作を扱えるように[aeval]の定義を拡張することは簡単には行きません。([ADiv (ANum 5) (ANum 0)]の結果何を返すべきでしょうか？)
 しかし、[aevalR]を拡張することは簡単です。*)
 
+Reserved Notation "e '\\' n"
+                  (at level 50, left associativity).
+
 Inductive aevalR : aexp -> nat -> Prop :=
   | E_ANum : forall (n:nat),
-      (ANum n) || n
+      (ANum n) \\ n
   | E_APlus : forall (a1 a2: aexp) (n1 n2 : nat),
-      (a1 || n1) -> (a2 || n2) -> (APlus a1 a2) || (n1 + n2)
+      (a1 \\ n1) -> (a2 \\ n2) -> (APlus a1 a2) \\ (n1 + n2)
   | E_AMinus : forall (a1 a2: aexp) (n1 n2 : nat),
-      (a1 || n1) -> (a2 || n2) -> (AMinus a1 a2) || (n1 - n2)
+      (a1 \\ n1) -> (a2 \\ n2) -> (AMinus a1 a2) \\ (n1 - n2)
   | E_AMult :  forall (a1 a2: aexp) (n1 n2 : nat),
-      (a1 || n1) -> (a2 || n2) -> (AMult a1 a2) || (n1 * n2)
+      (a1 \\ n1) -> (a2 \\ n2) -> (AMult a1 a2) \\ (n1 * n2)
   | E_ADiv :  forall (a1 a2: aexp) (n1 n2 n3: nat),
-      (a1 || n1) -> (a2 || n2) -> (mult n2 n3 = n1) -> (ADiv a1 a2) || n3
+      (a1 \\ n1) -> (a2 \\ n2) -> (n2 > 0) ->
+      (mult n2 n3 = n1) -> (ADiv a1 a2) \\ n3
 
-where "a '||' n" := (aevalR a n) : type_scope.
+where "a '\\' n" := (aevalR a n) : type_scope.
 
 End aevalR_division.
+
 Module aevalR_extended.
 
+(*  *** Adding Nondeterminism *)
+(** *** 非決定性の追加 *)
 
 (*  Suppose, instead, that we want to extend the arithmetic operations
-    by a nondeterministic number generator [any]:*)
-(** そのかわりに、非決定的な数の生成元である[any]を加えて、計算操作を拡張したいと思ったとします。*)
+    by a nondeterministic number generator [any] that, when evaluated,
+    may yield any number.  (Note that this is not the same as making a
+    _probabilistic_ choice among all possible numbers -- we're not
+    specifying any particular distribution of results, but just saying
+    what results are _possible_.) *)
+(** TODO そのかわりに、非決定的な数の生成元である[any]を加えて、計算操作を拡張したいと思ったとします。*)
+
+Reserved Notation "e '\\' n" (at level 50, left associativity).
+
 Inductive aexp : Type :=
   | AAny  : aexp                   (* <--- NEW *)
   | ANum : nat -> aexp
@@ -1211,20 +1160,21 @@ Inductive aexp : Type :=
 *)
 Inductive aevalR : aexp -> nat -> Prop :=
   | E_Any : forall (n:nat),
-      AAny || n                 (* <--- new *)
+      AAny \\ n                 (* <--- new *)
   | E_ANum : forall (n:nat),
-      (ANum n) || n
+      (ANum n) \\ n
   | E_APlus : forall (a1 a2: aexp) (n1 n2 : nat),
-      (a1 || n1) -> (a2 || n2) -> (APlus a1 a2) || (n1 + n2)
+      (a1 \\ n1) -> (a2 \\ n2) -> (APlus a1 a2) \\ (n1 + n2)
   | E_AMinus : forall (a1 a2: aexp) (n1 n2 : nat),
-      (a1 || n1) -> (a2 || n2) -> (AMinus a1 a2) || (n1 - n2)
+      (a1 \\ n1) -> (a2 \\ n2) -> (AMinus a1 a2) \\ (n1 - n2)
   | E_AMult :  forall (a1 a2: aexp) (n1 n2 : nat),
-      (a1 || n1) -> (a2 || n2) -> (AMult a1 a2) || (n1 * n2)
+      (a1 \\ n1) -> (a2 \\ n2) -> (AMult a1 a2) \\ (n1 * n2)
 
-where "a '||' n" := (aevalR a n) : type_scope.
+where "a '\\' n" := (aevalR a n) : type_scope.
 
 End aevalR_extended.
 
+(* ####################################################### *)
 (*  * Expressions With Variables *)
 (** * 変数を持つ式 *)
 
@@ -1236,149 +1186,39 @@ End aevalR_extended.
     算術式とブール式に変数を拡張することです。
     話を単純にするため、すべての変数はグローバルで、数値だけを持つとしましょう。 *)
 
-(* ##################################################### *)
-(*  ** Identifiers *)
-(** ** 識別子 *)
-
-(*  To begin, we'll need to formalize _identifiers_ such as program
-    variables.  We could use strings for this -- or, in a real
-    compiler, fancier structures like pointers into a symbol table.
-    But for simplicity let's just use natural numbers as identifiers. *)
-
-(*  (We hide this section in a module because these definitions are
-    actually in [SfLib], but we want to repeat them here so that we
-    can explain them.) *)
-(** 始めに、プログラム変数などの識別子(_identifiers_)を形式化しなければなりません。
-    このために文字列を使うこともできるでしょうし、(実際のコンパイラでは)
-    シンボルテーブルへのポインタのようなある種の特別な構造を使うこともできるでしょう。
-    しかし、簡単にするため、識別子に単に自然数を使います。
-
-    (このセクションをモジュールに隠します。それは、これらの定義が実際には[SfLib_J.v]
-    にあるからです。しかし説明のためにここで繰り返します。) *)
-
-Module Id. 
-
-(*  We define a new inductive datatype [Id] so that we won't confuse
-    identifiers and numbers.  We use [sumbool] to define a computable
-    equality operator on [Id]. *)
-(** 新しいデータタイプ[Id]を定義して、識別子と数値を混乱しないようにします。 
-   [Id]についての計算可能な同値演算子を定義するために、[sumbool]を使用します。*)
-
-Inductive id : Type :=
-  Id : nat -> id.
-
-Theorem eq_id_dec : forall id1 id2 : id, {id1 = id2} + {id1 <> id2}.
-Proof.
-   intros id1 id2.
-   destruct id1 as [n1]. destruct id2 as [n2].
-   destruct (eq_nat_dec n1 n2) as [Heq | Hneq].
-   Case "n1 = n2".
-     left. rewrite Heq. reflexivity.
-   Case "n1 <> n2".
-     right. intros contra. inversion contra. apply Hneq. apply H0.
-Defined. 
-
-(* The following lemmas will be useful for rewriting terms involving [eq_id_dec]. *)
-(** 次の補題は、[eq_id_dec]を含む式を書き直すのに役立ちます。 *)
-
-Lemma eq_id : forall (T:Type) x (p q:T), 
-              (if eq_id_dec x x then p else q) = p. 
-Proof.
-  intros. 
-  destruct (eq_id_dec x x). 
-  Case "x = x". 
-    reflexivity.
-  Case "x <> x (impossible)". 
-    apply ex_falso_quodlibet; apply n; reflexivity. Qed.
-
-(** **** Exercise: 1 star, optional (neq_id) *)
-Lemma neq_id : forall (T:Type) x y (p q:T), x <> y -> 
-               (if eq_id_dec x y then p else q) = q. 
-Proof.
-  (* FILL IN HERE *) Admitted.
-(** [] *)
-
-
-End Id. 
-
 (* ####################################################### *)
 (*  ** States *)
 (** ** 状態 *)
 
-(** A _state_ represents the current values of all the variables at
-    some point in the execution of a program. *)
-(** 状態(_state_)はプログラムの実行のある時点のすべての変数の現在値を表します。 *)
-(** For simplicity (to avoid dealing with partial functions), we
+(** Since we'll want to look variables up to find out their current
+    values, we'll reuse the type [id] from the [Maps] chapter for the
+    type of variables in Imp.
+
+    A _machine state_ (or just _state_) represents the current values
+    of _all_ variables at some point in the execution of a program. *)
+(** 
+TODO
+_マシン状態_(あるいは単に_状態_)はプログラムの実行のある時点のすべての変数の現在値を表します。 *)
+
+(** For simplicity, we assume that the state is defined for
+    _all_ variables, even though any given program is only going to
+    mention a finite number of them.  The state captures all of the
+    information stored in memory.  For Imp programs, because each
+    variable stores a natural number, we can represent the state as a
+    mapping from identifiers to [nat].  For more complex programming
+    languages, the state might have more structure. *)
+(TODO:
+(*  For simplicity (to avoid dealing with partial functions), we
     let the state be defined for _all_ variables, even though any
     given program is only going to mention a finite number of them. *)
 (** 簡単にするため(部分関数を扱うのを避けるため)、
     どのようなプログラムも有限個の変数しか使わないにもかかわらず、
     状態はすべての変数について値を定義しているものとします。 *)
 
-Definition state := id -> nat.
+Definition state := total_map nat.
 
 Definition empty_state : state :=
-  fun _ => 0.
-
-Definition update (st : state) (x : id) (n : nat) : state :=
-  fun x' => if eq_id_dec x x' then n else st x'.
-
-(** For proofs involving states, we'll need several simple properties
-    of [update]. *)
-(** 状態を含む証明のために、[update]についての単純な性質が必要です。 *)
-
-(*  **** Exercise: 1 star (update_eq) *)
-(** **** 練習問題: ★, optional (update_eq) *)
-Theorem update_eq : forall n x st,
-  (update st x n) x = n.
-Proof.
-  (* FILL IN HERE *) Admitted.
-(** [] *)
-
-(*  **** Exercise: 1 star (update_neq) *)
-(** **** 練習問題: ★, optional (update_neq) *)
-Theorem update_neq : forall x2 x1 n st,
-  x2 <> x1 ->                        
-  (update st x2 n) x1 = (st x1).
-Proof.
-  (* FILL IN HERE *) Admitted.
-(** [] *)
-
-(*  **** Exercise: 1 star (update_example) *)
-(** **** 練習問題: ★, optional (update_example) *)
-(** Before starting to play with tactics, make sure you understand
-    exactly what the theorem is saying! *)
-(** タクティックを使って遊び始める前に、
-    定理が言っていることを正確に理解していることを確認しなさい! *)
-
-Theorem update_example : forall (n:nat),
-  (update empty_state (Id 2) n) (Id 3) = 0.
-Proof.
-  (* FILL IN HERE *) Admitted.
-(** [] *)
-
-(** **** Exercise: 1 star (update_shadow) *)
-Theorem update_shadow : forall n1 n2 x1 x2 (st : state),
-   (update  (update st x2 n1) x2 n2) x1 = (update st x2 n2) x1.
-Proof.
-  (* FILL IN HERE *) Admitted.
-(** [] *)
-
-(** **** Exercise: 2 stars (update_same) *)
-Theorem update_same : forall n1 x1 x2 (st : state),
-  st x1 = n1 ->
-  (update st x1 n1) x2 = st x2.
-Proof.
-  (* FILL IN HERE *) Admitted.
-(** [] *)
-
-(** **** Exercise: 3 stars (update_permute) *)
-Theorem update_permute : forall n1 n2 x1 x2 x3 st,
-  x2 <> x1 -> 
-  (update (update st x2 n1) x1 n2) x3 = (update (update st x1 n2) x2 n1) x3.
-Proof.
-  (* FILL IN HERE *) Admitted.
-(** [] *)
+  t_empty 0.
 
 (* ################################################### *)
 (*  ** Syntax  *)
@@ -1387,7 +1227,6 @@ Proof.
 (*  We can add variables to the arithmetic expressions we had before by
     simply adding one more constructor: *)
 (** 前に定義した算術式に、単にもう1つコンストラクタを追加することで変数を追加できます: *)
-
 
 Inductive aexp : Type :=
   | ANum : nat -> aexp
@@ -1416,9 +1255,9 @@ Definition Z : id := Id 2.
     型に大文字の記号を使うという以前の使用法と衝突します。
     コースのこの部分では多相性を多用はしないので、このことが混乱を招くことはないはずです。) *)
 
-(** The definition of [bexp]s is the same as before (using the new
+(** The definition of [bexp]s is unchanged (except for using the new
     [aexp]s): *)
-(** [bexp]の定義は前と同じです(ただし新しい[aexp]を使います): *)
+(** [bexp]の定義は前と変更はありません(新しい[aexp]を使う点を除いて): *)
 
 Inductive bexp : Type :=
   | BTrue : bexp
@@ -1427,11 +1266,6 @@ Inductive bexp : Type :=
   | BLe : aexp -> aexp -> bexp
   | BNot : bexp -> bexp
   | BAnd : bexp -> bexp -> bexp.
-
-Tactic Notation "bexp_cases" tactic(first) ident(c) :=
-  first;
-  [ Case_aux c "BTrue" | Case_aux c "BFalse" | Case_aux c "BEq"
-  | Case_aux c "BLe" | Case_aux c "BNot" | Case_aux c "BAnd" ].
 
 (* ################################################### *)
 (*  ** Evaluation  *)
@@ -1455,19 +1289,19 @@ Fixpoint beval (st : state) (b : bexp) : bool :=
   | BTrue       => true
   | BFalse      => false
   | BEq a1 a2   => beq_nat (aeval st a1) (aeval st a2)
-  | BLe a1 a2   => ble_nat (aeval st a1) (aeval st a2)
+  | BLe a1 a2   => leb (aeval st a1) (aeval st a2)
   | BNot b1     => negb (beval st b1)
   | BAnd b1 b2  => andb (beval st b1) (beval st b2)
   end.
 
 Example aexp1 :
-  aeval (update empty_state X 5)
+  aeval (t_update empty_state X 5)
         (APlus (ANum 3) (AMult (AId X) (ANum 2)))
   = 13.
 Proof. reflexivity. Qed.
 
 Example bexp1 :
-  beval (update empty_state X 5)
+  beval (t_update empty_state X 5)
         (BAnd BTrue (BNot (BLe (AId X) (ANum 4))))
   = true.
 Proof. reflexivity. Qed.
@@ -1485,41 +1319,37 @@ Proof. reflexivity. Qed.
 (** ** 構文 *)
 
 (** Informally, commands [c] are described by the following BNF
-    grammar:
-     c ::= SKIP
-         | x ::= a
-         | c ; c
-         | WHILE b DO c END
-         | IFB b THEN c ELSE c FI
-    For example, here's the factorial function in Imp.
-     Z ::= X;
-     Y ::= 1;
-     WHILE not (Z = 0) DO
-       Y ::= Y * Z;
-       Z ::= Z - 1
-     END
-   When this command terminates, the variable [Y] will contain the
-   factorial of the initial value of [X].
-*)
-(** 非形式的には、コマンドは以下の BNF で表現されます。
+    grammar.  (We choose this slightly awkward concrete syntax for the
+    sake of being able to define Imp syntax using Coq's Notation
+    mechanism.  In particular, we use [IFB] to avoid conflicting with
+    the [if] notation from the standard library.) *)
+(** TODO 非形式的には、コマンドは以下の BNF で表現されます。
     構文:
-     c  ::= 'SKIP'
-         | X '::=' aexp
-         | c ';' c
-         | 'WHILE' bexp 'DO' c 'END'
-         | 'IFB' bexp 'THEN' c 'ELSE' c 'FI'
-    例えば、Imp における階乗関数は以下のようになります。
-     Z ::= X;
-     Y ::= 1;
+
+     c ::= SKIP | x ::= a | c ;; c | IFB b THEN c ELSE c FI 
+         | WHILE b DO c END
+
+*)
+(**
+    For example, here's factorial in Imp:
+
+     Z ::= X;;
+     Y ::= 1;;
      WHILE not (Z = 0) DO
-       Y ::= Y * Z;
+       Y ::= Y * Z;;
        Z ::= Z - 1
      END
+*)
+(*
+   When this command terminates, the variable [Y] will contain the
+   factorial of the initial value of [X]. *)
+(**
    このコマンドが終わったとき、変数 [Y] は変数 [X] の階乗の値を持つでしょう。
 *)
 
-(*  Here is the formal definition of the syntax of commands: *)
-(** 以下に、コマンドの構文の形式的な定義を示します。 *)
+(*  Here is the formal definition of the abstract syntax of
+    commands: *)
+(** 以下に、コマンドの抽象構文の形式的な定義を示します。 *)
 
 Inductive com : Type :=
   | CSkip : com
@@ -1528,11 +1358,6 @@ Inductive com : Type :=
   | CIf : bexp -> com -> com -> com
   | CWhile : bexp -> com -> com.
 
-Tactic Notation "com_cases" tactic(first) ident(c) :=
-  first;
-  [ Case_aux c "SKIP" | Case_aux c "::=" | Case_aux c ";;"
-  | Case_aux c "IFB" | Case_aux c "WHILE" ].
-
 (*  As usual, we can use a few [Notation] declarations to make things
     more readable.  We need to be a bit careful to avoid conflicts
     with Coq's built-in notations, so we'll keep this light -- in
@@ -1540,7 +1365,8 @@ Tactic Notation "com_cases" tactic(first) ident(c) :=
     [bexps] to avoid confusion with the numerical and boolean
     operators we've already defined.  We use the keyword [IFB] for
     conditionals instead of [IF], for similar reasons. *)
-(** いつものとおり、より読みやすいよう、いくつかの [Notation] 宣言が使えます。
+(** TODO !
+    いつものとおり、より読みやすいよう、いくつかの [Notation] 宣言が使えます。
     しかし、Coq の組み込みの表記と衝突しないよう、少し気をつける必要があります 
     (手軽さを維持しつつ！)。
     特に、[aexp] と [bexp] については、
@@ -1578,7 +1404,7 @@ Definition fact_in_coq : com :=
 (** ** 例 *)
 
 (*  Assignment: *)
-(** 割り当て: *)
+(** 代入: *)
 
 Definition plus2 : com :=
   X ::= (APlus (AId X) (ANum 2)).
@@ -1590,8 +1416,8 @@ Definition subtract_slowly_body : com :=
   Z ::= AMinus (AId Z) (ANum 1) ;;
   X ::= AMinus (AId X) (ANum 1).
 
-(*  Loops: *)
-(** ループ: *)
+(*  *** Loops: *)
+(** *** ループ: *)
 
 Definition subtract_slowly : com :=
   WHILE BNot (BEq (AId X) (ANum 0)) DO
@@ -1603,8 +1429,8 @@ Definition subtract_3_from_5_slowly : com :=
   Z ::= ANum 5 ;;
   subtract_slowly.
 
-(*  An infinite loop: *)
-(** 無限ループ: *)
+(*  *** An infinite loop: *)
+(** *** 無限ループ: *)
 
 Definition loop : com :=
   WHILE BTrue DO
@@ -1629,12 +1455,13 @@ Definition loop : com :=
     omitting the [WHILE] case. *)
 (** 以下は [WHILE] 以外のコマンドの評価関数を得ようとした、最初の試みです。 *)
 
-Fixpoint ceval_fun_no_while (st : state) (c : com) : state :=
+Fixpoint ceval_fun_no_while (st : state) (c : com)
+                          : state :=
   match c with
     | SKIP =>
         st
     | x ::= a1 =>
-        update st x (aeval st a1)
+        t_update st x (aeval st a1)
     | c1 ;; c2 =>
         let st' := ceval_fun_no_while st c1 in
         ceval_fun_no_while st' c2
@@ -1646,21 +1473,21 @@ Fixpoint ceval_fun_no_while (st : state) (c : com) : state :=
         st  (* bogus *)
   end.
 
-(* In a traditional functional programming language like ML or
-    Haskell we could write the [WHILE] case as follows:
-<<
+(*  In a traditional functional programming language like OCaml or
+    Haskell we could add the [WHILE] case as follows:
+
   Fixpoint ceval_fun (st : state) (c : com) : state :=
     match c with
       ...
       | WHILE b DO c END =>
-          if (beval st b1)
-            then ceval_fun st (c1; WHILE b DO c END)
+          if (beval st b)
+            then ceval_fun st (c; WHILE b DO c END)
             else st
     end.
->>
+
     Coq doesn't accept such a definition ("Error: Cannot guess
     decreasing argument of fix") because the function we want to
-    define is not guaranteed to terminate. Indeed, it doesn't always
+    define is not guaranteed to terminate. Indeed, it _doesn't_ always
     terminate: for example, the full version of the [ceval_fun]
     function applied to the [loop] program above would never
     terminate. Since Coq is not just a functional programming
@@ -1668,18 +1495,19 @@ Fixpoint ceval_fun_no_while (st : state) (c : com) : state :=
     non-terminating function needs to be rejected. Here is
     an (invalid!) Coq program showing what would go wrong if Coq
     allowed non-terminating recursive functions:
-<<
-     Fixpoint loop_false (n : nat) : False := loop_false n.
->>
+
+         Fixpoint loop_false (n : nat) : False := loop_false n.
+
     That is, propositions like [False] would become provable
-    (e.g. [loop_false 0] would be a proof of [False]), which
+    (e.g., [loop_false 0] would be a proof of [False]), which
     would be a disaster for Coq's logical consistency.
 
     Thus, because it doesn't terminate on all inputs, the full version
     of [ceval_fun] cannot be written in Coq -- at least not without
-    additional tricks (see chapter [ImpCEvalFun] if curious). *)
-(** MLやHaskellといった伝統的な関数型プログラム言語において、[WHILE]は以下のように書けます。 
-<<
+    additional tricks (see chapter [ImpCEvalFun] if you're curious 
+    about what those might be). *)
+(** OCamlやHaskellといった伝統的な関数型プログラム言語において、[WHILE]は以下のように書けます。 
+
   Fixpoint ceval_fun (st : state) (c : com) : state :=
     match c with
       ...
@@ -1688,29 +1516,30 @@ Fixpoint ceval_fun_no_while (st : state) (c : com) : state :=
             then ceval_fun st (c1; WHILE b DO c END)
             else st
     end.
->>
+
    Coqはそのような定義を受け入れてはくれません。("Error: Cannot gess decreasing argument of fix" というエラーになります。)
    我々が定義したい関数は、終了を保証しないからです。実際に必ずしも終了しません：
    たとえば、[ceval_fun]の完全なバージョンは、上記の[loop]プログラムを適用した場合、決して終了しません。
    Coqは関数型プログラミング言語であるだけではなく、一貫した論理そのものであり、終了しない可能性のある関数は排除されなければならないのです。  
    ここに、もしCoqが終了しない帰納的な関数を許す場合に、どんなおかしなことが起こるかを示す(間違った)Coqのプログラムをあげておきます。
-<<
+
      Fixpoint loop_false (n : nat) : False := loop_false n.
->>
+
   すなわち、[False]のような命題が証明可能になってしまします。。(例として、[loop_false 0]は[False]であることの証明である。というように。)
   Coqの論理的一貫性にとってやっかいなことです。
   
   それゆえ、すべての入力について終了が保証出来ないので、[ceval_fun]は決してCoqで書くことが出来ないのです。 -- 少なくとも追加のトリックなしには。
   (気になるなら、[ImpCEvalFun]の章を見てください。)
+  TODO
 *)
 
 (* #################################### *)
 (*  ** Evaluation as a Relation *)
 (** * 関係としての評価 *)
 
-(* Here's a better way: we define [ceval] as a _relation_ rather than
-    a _function_ -- i.e., we define it in [Prop] instead of [Type], as
-    we did for [aevalR] above. *)
+(*  Here's a better way: define [ceval] as a _relation_ rather than a
+    _function_ -- i.e., define it in [Prop] instead of [Type], as we
+    did for [aevalR] above. *)
 (** ここに改善策があります: [ceval] を関数ではなく関係 (relation) として定義しましょう。
     つまり、上の aevalR と bevalR と同様に Type ではなく Prop で定義しましょう。 *)
 
@@ -1723,89 +1552,87 @@ Fixpoint ceval_fun_no_while (st : state) (c : com) : state :=
     partial function! *)
 (** これは重要な変更です。 ステップ指数をすべての場所で引き回す馬鹿馬鹿しさから解放してくれるのに加え、 
     定義での柔軟性を与えてくれます。 例えば、もし言語に並行性の要素を導入したら、評価の定義を非決定的に書きたくなるでしょう。
-    つまり、その関数は全関数でないだけでなく、部分関数ですらないかも知れません！ *)
+    つまり、その関数は全関数でないだけでなく、部分関数ですらないかも知れません！
+    TODO
+    *)
 
 
-(*  We'll use the notation [c / st || st'] for our [ceval] relation:
-    [c / st || st'] means that executing program [c] in a starting
+(*  We'll use the notation [c / st \\ st'] for our [ceval] relation:
+    [c / st \\ st'] means that executing program [c] in a starting
     state [st] results in an ending state [st'].  This can be
     pronounced "[c] takes state [st] to [st']". *)
 (** ceavl 関係に対する表記として c / st ⇓ st' を使います。
-    正確に言うと、c / st || st' と書いたらプログラム c を初期状態 st で評価すると、 
+    正確に言うと、c / st \\ st' と書いたらプログラム c を初期状態 st で評価すると、 
     その結果は最終状態 st' になる、ということを意味します。 これは「c は状態 st を st' に持っていく」とも言えます。 
                            ----------------                            (E_Skip)
-                           SKIP / st || st
+                           SKIP / st \\ st
 
                            aeval st a1 = n
                    --------------------------------                     (E_Ass)
-                   x := a1 / st || (update st x n)
+                   x := a1 / st \\ (t_update st x n)
 
-                           c1 / st || st'
-                          c2 / st' || st''
+                           c1 / st \\ st'
+                          c2 / st' \\ st''
                          -------------------                            (E_Seq)
-                         c1;;c2 / st || st''
+                         c1;;c2 / st \\ st''
 
                           beval st b1 = true
-                           c1 / st || st'
+                           c1 / st \\ st'
                 -------------------------------------                (E_IfTrue)
-                IF b1 THEN c1 ELSE c2 FI / st || st'
+                IF b1 THEN c1 ELSE c2 FI / st \\ st'
 
                          beval st b1 = false
-                           c2 / st || st'
+                           c2 / st \\ st'
                 -------------------------------------               (E_IfFalse)
-                IF b1 THEN c1 ELSE c2 FI / st || st'
+                IF b1 THEN c1 ELSE c2 FI / st \\ st'
 
-                         beval st b1 = false
+                         beval st b = false
                     ------------------------------                 (E_WhileEnd)
-                    WHILE b DO c END / st || st
+                    WHILE b DO c END / st \\ st
 
-                          beval st b1 = true
-                           c / st || st'
-                  WHILE b DO c END / st' || st''
+                          beval st b = true
+                           c / st \\ st'
+                  WHILE b DO c END / st' \\ st''
                   ---------------------------------               (E_WhileLoop)
-                    WHILE b DO c END / st || st''
+                    WHILE b DO c END / st \\ st''
+
 *)
 
-(*  Here is the formal definition.  (Make sure you understand
-    how it corresponds to the inference rules.) *)
-(** 以下に形式的な定義を挙げます。 (上の推論規則とどのように対応するか、確認しておきましょう。)  *)
+(*  Here is the formal definition.  Make sure you understand
+    how it corresponds to the inference rules. *)
+(** 以下に形式的な定義を挙げます。 上の推論規則とどのように対応するか、確認しておきましょう。  *)
 
-Reserved Notation "c1 '/' st '||' st'" (at level 40, st at level 39).
+Reserved Notation "c1 '/' st '\\' st'"
+                  (at level 40, st at level 39).
 
 Inductive ceval : com -> state -> state -> Prop :=
   | E_Skip : forall st,
-      SKIP / st || st
+      SKIP / st \\ st
   | E_Ass  : forall st a1 n x,
       aeval st a1 = n ->
-      (x ::= a1) / st || (update st x n)
+      (x ::= a1) / st \\ (t_update st x n)
   | E_Seq : forall c1 c2 st st' st'',
-      c1 / st  || st' ->
-      c2 / st' || st'' ->
-      (c1 ;; c2) / st || st''
+      c1 / st  \\ st' ->
+      c2 / st' \\ st'' ->
+      (c1 ;; c2) / st \\ st''
   | E_IfTrue : forall st st' b c1 c2,
       beval st b = true ->
-      c1 / st || st' ->
-      (IFB b THEN c1 ELSE c2 FI) / st || st'
+      c1 / st \\ st' ->
+      (IFB b THEN c1 ELSE c2 FI) / st \\ st'
   | E_IfFalse : forall st st' b c1 c2,
       beval st b = false ->
-      c2 / st || st' ->
-      (IFB b THEN c1 ELSE c2 FI) / st || st'
+      c2 / st \\ st' ->
+      (IFB b THEN c1 ELSE c2 FI) / st \\ st'
   | E_WhileEnd : forall b st c,
       beval st b = false ->
-      (WHILE b DO c END) / st || st
+      (WHILE b DO c END) / st \\ st
   | E_WhileLoop : forall st st' st'' b c,
       beval st b = true ->
-      c / st || st' ->
-      (WHILE b DO c END) / st' || st'' ->
-      (WHILE b DO c END) / st || st''
+      c / st \\ st' ->
+      (WHILE b DO c END) / st' \\ st'' ->
+      (WHILE b DO c END) / st \\ st''
 
-  where "c1 '/' st '||' st'" := (ceval c1 st st').
-
-Tactic Notation "ceval_cases" tactic(first) ident(c) :=
-  first;
-  [ Case_aux c "E_Skip" | Case_aux c "E_Ass" | Case_aux c "E_Seq"
-  | Case_aux c "E_IfTrue" | Case_aux c "E_IfFalse"
-  | Case_aux c "E_WhileEnd" | Case_aux c "E_WhileLoop" ].
+  where "c1 '/' st '\\' st'" := (ceval c1 st st').
 
 (*  The cost of defining evaluation as a relation instead of a
     function is that we now need to construct _proofs_ that some
@@ -1813,6 +1640,7 @@ Tactic Notation "ceval_cases" tactic(first) ident(c) :=
     Coq's computation mechanism do it for us. *)
 (** 評価を関数ではなく関係として定義することのコストは、 あるプログラムを実行した結果がとある状態になる、 
     というのを Coq の計算機構にやってもらうだけではなく、 その「証明」を構築する必要がある、ということです。 *)
+
 Example ceval_example1:
     (X ::= ANum 2;;
      IFB BLe (AId X) (ANum 1)
@@ -1820,13 +1648,13 @@ Example ceval_example1:
        ELSE Z ::= ANum 4
      FI)
    / empty_state
-   || (update (update empty_state X 2) Z 4).
+   \\ (t_update (t_update empty_state X 2) Z 4).
 Proof.
   (* We must supply the intermediate state *)
-  apply E_Seq with (update empty_state X 2).
-  Case "assignment command".
+  apply E_Seq with (t_update empty_state X 2).
+  - (* assignment command *)
     apply E_Ass. reflexivity.
-  Case "if command".
+  - (* if command *)
     apply E_IfFalse.
       reflexivity.
       apply E_Ass. reflexivity.  Qed.
@@ -1834,8 +1662,8 @@ Proof.
 (* **** Exercise: 2 stars (ceval_example2) *)
 (** **** 練習問題: ★★(ceval_example2) *)
 Example ceval_example2:
-    (X ::= ANum 0;; Y ::= ANum 1;; Z ::= ANum 2) / empty_state ||
-    (update (update (update empty_state X 0) Y 1) Z 2).
+    (X ::= ANum 0;; Y ::= ANum 1;; Z ::= ANum 2) / empty_state \\
+    (t_update (t_update (t_update empty_state X 0) Y 1) Z 2).
 Proof.
   (* FILL IN HERE *) Admitted.
 (** [] *)
@@ -1844,8 +1672,8 @@ Proof.
 (** **** 練習問題: ★★★, advanced (pup_to_n) *)
 (* Write an Imp program that sums the numbers from [1] to
    [X] (inclusive: [1 + 2 + ... + X]) in the variable [Y].
-   Prove that this program executes as intended for X = 2
-   (this latter part is trickier than you might expect). *)
+   Prove that this program executes as intended for [X] = [2]
+   (the latter is trickier than you might expect). *)
 (** [1]からXまでの数を合計([1 + 2 + ... + X]を含みます)して、変数Yに結果を格納するImpプログラムを書きなさい。
     このプログラムがX = 2のときに意図したとおりに動くことを証明しなさい。
     後の問題はあなたが考えているよりもトリッキーかもしれません*)
@@ -1854,8 +1682,8 @@ Definition pup_to_n : com :=
   (* FILL IN HERE *) admit.
 
 Theorem pup_to_2_ceval :
-  pup_to_n / (update empty_state X 2) ||
-    update (update (update (update (update (update empty_state
+  pup_to_n / (t_update empty_state X 2) \\
+    t_update (t_update (t_update (t_update (t_update (t_update empty_state
       X 2) Y 0) Y 2) X 1) Y 3) X 0.
 Proof.
   (* FILL IN HERE *) Admitted.
@@ -1878,7 +1706,8 @@ Proof.
 
     In fact, this cannot happen: [ceval] is a partial function.
     Here's the proof: *)
-(** 評価の定義を計算的なものから関係的なものに変更するのは、
+(** TODO
+評価の定義を計算的なものから関係的なものに変更するのは、
     評価は全関数であるべきという (Fixpoint の定義における 
     Coq の制限によって課せられる) 不自然な要求から逃れさせてくれる良い変更です。
     しかしこれは、2 つ目の評価の定義は本当に部分関数なのか？という疑問ももたらします。
@@ -1889,42 +1718,38 @@ Proof.
    以下に証明を挙げます: *)
 
 Theorem ceval_deterministic: forall c st st1 st2,
-     c / st || st1  ->
-     c / st || st2 ->
+     c / st \\ st1  ->
+     c / st \\ st2 ->
      st1 = st2.
 Proof.
   intros c st st1 st2 E1 E2.
   generalize dependent st2.
-  ceval_cases (induction E1) Case;
+  induction E1;
            intros st2 E2; inversion E2; subst.
-  Case "E_Skip". reflexivity.
-  Case "E_Ass". reflexivity.
-  Case "E_Seq".
+  - (* E_Skip *) reflexivity.
+  - (* E_Ass *) reflexivity.
+  - (* E_Seq *)
     assert (st' = st'0) as EQ1.
-      SCase "Proof of assertion". apply IHE1_1; assumption.
+    { (* Proof of assertion *) apply IHE1_1; assumption. }
     subst st'0.
     apply IHE1_2. assumption.
-  Case "E_IfTrue".
-    SCase "b1 evaluates to true".
+  - (* E_IfTrue, b1 evaluates to true *)
       apply IHE1. assumption.
-    SCase "b1 evaluates to false (contradiction)".
+  - (* E_IfTrue,  b1 evaluates to false (contradiction) *)
       rewrite H in H5. inversion H5.
-  Case "E_IfFalse".
-    SCase "b1 evaluates to true (contradiction)".
-      rewrite H in H5. inversion H5.
-    SCase "b1 evaluates to false".
+  - (* E_IfFalse, b1 evaluates to true (contradiction) *)
+    rewrite H in H5. inversion H5.
+  - (* E_IfFalse, b1 evaluates to false *)
       apply IHE1. assumption.
-  Case "E_WhileEnd".
-    SCase "b1 evaluates to false".
-      reflexivity.
-    SCase "b1 evaluates to true (contradiction)".
-      rewrite H in H2. inversion H2.
-  Case "E_WhileLoop".
-    SCase "b1 evaluates to false (contradiction)".
-      rewrite H in H4. inversion H4.
-    SCase "b1 evaluates to true".
+  - (* E_WhileEnd, b1 evaluates to false *)
+    reflexivity.
+  - (* E_WhileEnd, b1 evaluates to true (contradiction) *)
+    rewrite H in H2. inversion H2.
+  - (* E_WhileLoop, b1 evaluates to false (contradiction) *)
+    rewrite H in H4. inversion H4.
+  - (* E_WhileLoop, b1 evaluates to true *)
       assert (st' = st'0) as EQ1.
-        SSCase "Proof of assertion". apply IHE1_1; assumption.
+      { (* Proof of assertion *) apply IHE1_1; assumption. }
       subst st'0.
       apply IHE1_2. assumption.  Qed.
 
@@ -1941,20 +1766,22 @@ Proof.
 
 (* This section explores some examples. *)
 (** このセクションで、いくつか例を見ていきましょう *)
+
 Theorem plus2_spec : forall st n st',
   st X = n ->
-  plus2 / st || st' ->
+  plus2 / st \\ st' ->
   st' X = n + 2.
 Proof.
   intros st n st' HX Heval.
-  (* Inverting Heval essentially forces Coq to expand one
-     step of the ceval computation - in this case revealing
-     that st' must be st extended with the new value of X,
-     since plus2 is an assignment *)
+  (* Inverting [Heval] essentially forces Coq to expand one step of
+     the ceval computation -- in this case revealing that [st']
+     must be [st] extended with the new value of [X], since plus2
+     is an assignment *)
   (* Hevalをinvertすることは本質的には、Coqにcevalの計算の一ステップを展開させることと同じです。
      このケースにおいては、plus2は代入であるため、st'がXの新しい値でstに拡大されることが明らかになります。*)
+
   inversion Heval. subst. clear Heval. simpl.
-  apply update_eq.  Qed.
+  apply t_update_eq.  Qed.
 
 (*  **** Exercise: 3 stars (XtimesYinZ_spec) *)
 (** **** 練習問題: ★★★, recommended (XtimesYinZ_spec) *)
@@ -1966,7 +1793,7 @@ Proof.
 
 (** **** Exercise: 3 stars (loop_never_stops) *)
 Theorem loop_never_stops : forall st st',
-  ~(loop / st || st').
+  ~(loop / st \\ st').
 Proof.
   intros st st' contra. unfold loop in contra.
   remember (WHILE BTrue DO SKIP END) as loopdef eqn:Heqloopdef.
@@ -2032,15 +1859,15 @@ Proof.
 (*  HP Calculators, programming languages like Forth and Postscript,
     and abstract machines like the Java Virtual Machine all evaluate
     arithmetic expressions using a stack. For instance, the expression
-<<
-   (2*3)+(3*(4-2))
->>
+
+      (2*3)+(3*(4-2))
+
    would be entered as
-<<
-   2 3 * 3 4 2 - * +
->>
+
+      2 3 * 3 4 2 - * +
+
    and evaluated like this:
-<<
+
   []            |    2 3 * 3 4 2 - * +
   [2]           |    3 * 3 4 2 - * +
   [3, 2]        |    * 3 4 2 - * +
@@ -2144,7 +1971,7 @@ Example s_execute1 :
 (* FILL IN HERE *) Admitted.
 
 Example s_execute2 :
-     s_execute (update empty_state X 3) [3;4]
+     s_execute (t_update empty_state X 3) [3;4]
        [SPush 4; SLoad X; SMult; SPlus]
    = [15; 4].
 (* FILL IN HERE *) Admitted.
@@ -2278,18 +2105,18 @@ Inductive status : Type :=
   | SContinue : status
   | SBreak : status.
 
-Reserved Notation "c1 '/' st '||' s '/' st'"
+Reserved Notation "c1 '/' st '\\' s '/' st'"
                   (at level 40, st, s at level 39).
 
-(** Intuitively, [c / st || s / st'] means that, if [c] is started in
+(** Intuitively, [c / st \\ s / st'] means that, if [c] is started in
     state [st], then it terminates in state [st'] and either signals
     that any surrounding loop (or the whole program) should exit
     immediately ([s = SBreak]) or that execution should continue
     normally ([s = SContinue]).
 
-    The definition of the "[c / st || s / st']" relation is very
+    The definition of the "[c / st \\ s / st']" relation is very
     similar to the one we gave above for the regular evaluation
-    relation ([c / st || s / st']) -- we just need to handle the
+    relation ([c / st \\ s / st']) -- we just need to handle the
     termination signals appropriately:
 
     - If the command is [SKIP], then the state doesn't change, and
@@ -2302,30 +2129,30 @@ Reserved Notation "c1 '/' st '||' s '/' st'"
       that variable in the state accordingly and signal that execution
       can continue normally.
 
-    - If the command is of the form [IF b THEN c1 ELSE c2 FI], then
+    - If the command is of the form [IFB b THEN c1 ELSE c2 FI], then
       the state is updated as in the original semantics of Imp, except
       that we also propagate the signal from the execution of
       whichever branch was taken.
 
-    - If the command is a sequence [c1 ; c2], we first execute
-      [c1]. If this yields a [SBreak], we skip the execution of [c2]
+    - If the command is a sequence [c1 ;; c2], we first execute
+      [c1].  If this yields a [SBreak], we skip the execution of [c2]
       and propagate the [SBreak] signal to the surrounding context;
-      the resulting state should be the same as the one obtained by
+      the resulting state is the same as the one obtained by
       executing [c1] alone. Otherwise, we execute [c2] on the state
-      obtained after executing [c1], and propagate the signal that was
+      obtained after executing [c1], and propagate the signal 
       generated there.
 
     - Finally, for a loop of the form [WHILE b DO c END], the
       semantics is almost the same as before. The only difference is
       that, when [b] evaluates to true, we execute [c] and check the
-      signal that it raises. If that signal is [SContinue], then the
+      signal that it raises.  If that signal is [SContinue], then the
       execution proceeds as in the original semantics. Otherwise, we
       stop the execution of the loop, and the resulting state is the
       same as the one resulting from the execution of the current
-      iteration. In either case, since [BREAK] only terminates the
+      iteration.  In either case, since [BREAK] only terminates the
       innermost loop, [WHILE] signals [SContinue]. *)
-(** 直感的に、[c / st || s / st']は次のことを意味します。もし、[c]が状態[st]で開始しているならば、それは状態[st']で終了し、囲まれているループ(またはプログラム全体)に対し直ちに([s=SBreak]の場合)終了するか、実行を正常どおり([s = SContinue]の場合)続けるかシグナルを出します。
-  "[c / st || s / st']" 関係の定義は、上記で通常の関係の評価として我々が与えた一つ	([c / st || s / st']) にとてもよく似ています。 -- 必要になるのは、終了シグナルを適切にハンドルすることだけです。
+(** 直感的に、[c / st \\ s / st']は次のことを意味します。もし、[c]が状態[st]で開始しているならば、それは状態[st']で終了し、囲まれているループ(またはプログラム全体)に対し直ちに([s=SBreak]の場合)終了するか、実行を正常どおり([s = SContinue]の場合)続けるかシグナルを出します。
+  "[c / st \\ s / st']" 関係の定義は、上記で通常の関係の評価として我々が与えた一つ	([c / st \\ s / st']) にとてもよく似ています。 -- 必要になるのは、終了シグナルを適切にハンドルすることだけです。
    
 *)    
     - [SKIP]コマンドの場合、状態は変更されませんし、どんな外部ループも正常に実行を続けることが出来ます。
@@ -2347,10 +2174,10 @@ Reserved Notation "c1 '/' st '||' s '/' st'"
 
 Inductive ceval : com -> state -> status -> state -> Prop :=
   | E_Skip : forall st,
-      CSkip / st || SContinue / st
+      CSkip / st \\ SContinue / st
   (* FILL IN HERE *)
 
-  where "c1 '/' st '||' s '/' st'" := (ceval c1 st s st').
+  where "c1 '/' st '\\' s '/' st'" := (ceval c1 st s st').
 
 Tactic Notation "ceval_cases" tactic(first) ident(c) :=
   first;
@@ -2361,38 +2188,38 @@ Tactic Notation "ceval_cases" tactic(first) ident(c) :=
 (*  Now the following properties of your definition of [ceval]: *)
 (** あなたの[ceval]の定義が次の性質を満たしているか確認しなさい *)
 Theorem break_ignore : forall c st st' s,
-     (BREAK;; c) / st || s / st' ->
+     (BREAK;; c) / st \\ s / st' ->
      st = st'.
 Proof.
   (* FILL IN HERE *) Admitted.
 
 Theorem while_continue : forall b c st st' s,
-  (WHILE b DO c END) / st || s / st' ->
+  (WHILE b DO c END) / st \\ s / st' ->
   s = SContinue.
 Proof.
   (* FILL IN HERE *) Admitted.
 
 Theorem while_stops_on_break : forall b c st st',
   beval st b = true ->
-  c / st || SBreak / st' ->
-  (WHILE b DO c END) / st || SContinue / st'.
+  c / st \\ SBreak / st' ->
+  (WHILE b DO c END) / st \\ SContinue / st'.
 Proof.
   (* FILL IN HERE *) Admitted.
 
 (*  **** Exercise: 3 stars, advanced, optional (while_break_true)  *)
 (** **** 練習問題: ★★★, advanced, optional (while_break_true)  *)
 Theorem while_break_true : forall b c st st',
-  (WHILE b DO c END) / st || SContinue / st' ->
+  (WHILE b DO c END) / st \\ SContinue / st' ->
   beval st' b = true ->
-  exists st'', c / st'' || SBreak / st'.
+  exists st'', c / st'' \\ SBreak / st'.
 Proof.
 (* FILL IN HERE *) Admitted.
 
 (*  **** Exercise: 4 stars, advanced, optional (ceval_deterministic)  *)
 (** **** 練習問題: ★★★★, advanced, optional (ceval_deterministic)  *)
 Theorem ceval_deterministic: forall (c:com) st st1 st2 s1 s2,
-     c / st || s1 / st1  ->
-     c / st || s2 / st2 ->
+     c / st \\ s1 / st1  ->
+     c / st \\ s2 / st2 ->
      st1 = st2 /\ s1 = s2.
 Proof.
   (* FILL IN HERE *) Admitted.
@@ -2427,7 +2254,7 @@ End BreakImp.
 
 (*  **** Exercise: 4 stars, optional (add_for_loop) *)
 (** **** 練習問題: ★★★★, optional (add_for_loop) *)
-(* Add C-style [for] loops to the language of commands, update the
+(*  Add C-style [for] loops to the language of commands, update the
     [ceval] definition to define the semantics of [for] loops, and add
     cases for [for] loops as needed so that all the proofs in this file
     are accepted by Coq.
@@ -2455,6 +2282,4 @@ End BreakImp.
 (* FILL IN HERE *)
 (** [] *)
 
-
-(* <$Date: 2013-07-17 16:19:11 -0400 (Wed, 17 Jul 2013) $ *)
-
+(* $Date: 2016-05-26 16:17:19 -0400 (Thu, 26 May 2016) $ *)
